CR and METCR reductions for HtS in ROM.

proofs/Cleanup/HashThenSign.ec
@@ -220,17 +220,17 @@ module type Adv_CR_RO(HO : POracle) = {
 
 module CR_RO(A : Adv_CR_RO, HO : Oracle) = {
   proc main() = {
-    var x, x' : rco_t * msg_al_t;
+    var kx, kx' : rco_t * msg_al_t;
     var y, y' : msg_fl_t;
     
     HO.init();
     
-    (x, x') <@ A(HO).find();
+    (kx, kx') <@ A(HO).find();
     
-    y <@ HO.o(x);
-    y' <@ HO.o(x');
+    y <@ HO.o(kx);
+    y' <@ HO.o(kx');
     
-    return x <> x' /\ y = y';
+    return kx <> kx' /\ y = y';
   }
 }.
 
@@ -285,24 +285,24 @@ module type Adv_METCR_RO(O : TOracle_METCR, HO : POracle) = {
 
 module M_ETCR_RO(A : Adv_METCR_RO, O : Oracle_METCR, HO : Oracle) = {
   proc main() = {
-    var rco, rco' : rco_t;
-    var mal, mal' : msg_al_t;
-    var mfl, mfl' : msg_fl_t;
+    var k, k' : rco_t;
+    var x, x' : msg_al_t;
+    var y, y' : msg_fl_t;
     var i, nrts : int;
     
     O.init();
     HO.init();
     
-    (i, rco', mal') <@ A(O, HO).find();
+    (i, k', x') <@ A(O, HO).find();
     
-    (rco, mal) <@ O.get(i);
+    (k, x) <@ O.get(i);
     
-    mfl <@ HO.o((rco, mal));
-    mfl' <@ HO.o((rco', mal'));
+    y <@ HO.o((k, x));
+    y' <@ HO.o((k', x'));
     
     nrts <@ O.nr_targets();
     
-    return 0 <= i < nrts /\ mal <> mal' /\ mfl = mfl';
+    return 0 <= i < nrts /\ x <> x' /\ y = y';
   }
 }.
 
@@ -367,7 +367,7 @@ module (R_EFCMARO_CRRO (FL_KU_DSS : FL_KU.Scheme, A : Adv_EFCMA_RO) : Adv_CR_RO)
       
       rco <$ drco;
 
-      cm <@ MCO.o((rco, m));
+      cm <@ HO.o((rco, m));
 
       (sigfl, sk) <@ FL_KU_DSS.sign(sk, cm);
 
@@ -403,10 +403,70 @@ module (R_EFCMARO_CRRO (FL_KU_DSS : FL_KU.Scheme, A : Adv_EFCMA_RO) : Adv_CR_RO)
   }
 }.  
 
-section Proof_EFCMA_RO_ALKUDSS.
-declare module FL_KU_DSS <: FL_KU.Scheme.
+search assoc onth. search map zip.
+module (R_EFCMARO_METCRRO (FL_KU_DSS : FL_KU.Scheme, A : Adv_EFCMA_RO) : Adv_METCR_RO) (O : TOracle_METCR, HO : POracle) = {
+  module O_CMA_R_EFCMARO_METCRRO : SOracle_CMA  = {
+    var sk : sk_al_t
+    var comps : (msg_fl_t * (rco_t * msg_al_t)) list
+    
+    proc init(sk_init : sk_al_t) = {
+      sk <- sk_init;
+      comps <- [];
+    }
+    
+    proc sign(m : msg_al_t) : sig_al_t = {
+      var rco : rco_t;
+      var cm : msg_fl_t;
+      var sigfl : sig_fl_t;
+      var sig : sig_al_t;
+      
+      rco <@ O.query(m);
 
-declare module A <: Adv_EFCMA_RO.
+      cm <@ HO.o((rco, m));
+
+      (sigfl, sk) <@ FL_KU_DSS.sign(sk, cm);
+
+      sig <- (rco, sigfl);
+
+      comps <- rcons comps (cm, (rco, m));
+            
+      return sig;
+    }
+  }
+  
+  proc find() : int * rco_t * msg_al_t = {
+    var pk : pk_al_t;
+    var sk : sk_al_t;
+    var rco, rco' : rco_t;
+    var mal, mal' : msg_al_t;
+    var sig' : sig_al_t;
+    var mfl' : msg_fl_t;
+    var i : int;
+    
+    (pk, sk) <@ AL_KU_DSS(FL_KU_DSS).keygen();
+    
+    O_CMA_R_EFCMARO_METCRRO.init(sk);
+    
+    (mal', sig') <@ A(O_CMA_R_EFCMARO_METCRRO, HO).forge(pk);
+    
+    rco' <- sig'.`1;
+    
+    mfl' <@ HO.o((rco', mal'));
+    
+    i <- index mfl' (unzip1 O_CMA_R_EFCMARO_METCRRO.comps);
+    
+    return (i, rco', mal');
+  }
+}.  
+
+
+
+section Proof_EFCMA_RO_ALKUDSS.
+
+declare module FL_KU_DSS <: FL_KU.Scheme{-ERO, -O_CMA, -O_METCR, -R_EFCMARO_CRRO, -R_EFCMARO_METCRRO}.
+declare axiom FL_KU_DSS_verify_ll : islossless FL_KU_DSS.verify. 
+
+declare module A <: Adv_EFCMA_RO{-FL_KU_DSS, -ERO, -O_CMA, -O_METCR, -R_EFCMARO_CRRO, -R_EFCMARO_METCRRO}.
 
 (* Signature queries *)
 declare op qS : { int | 0 <= qS } as ge0_qS.
@@ -414,5 +474,234 @@ declare op qS : { int | 0 <= qS } as ge0_qS.
 (* Random Oracle (Hash) queries *)
 declare op qH : { int | 0 <= qH } as ge0_qH.  
 
+
+local module O_CMA_Coll = {
+    var sk : sk_al_t
+    var qs : msg_al_t list
+    var comps : (msg_fl_t * (rco_t * msg_al_t)) list 
+        
+    (* Initialize secret/signing key and oracle query list qs *)
+    proc init(sk_init : sk_al_t) : unit = {
+      sk <- sk_init;
+      qs <- [];
+      comps <- [];
+    }
+
+    (* 
+      Sign given message m using the considered signature scheme with the
+      secret/signing key sk and append m to the list of oracle queries qs
+    *)
+    proc sign(m : msg_al_t) : sig_al_t = {
+      var rco : rco_t;
+      var cm : msg_fl_t;
+      var sigfl : sig_fl_t;
+      var sig : sig_al_t;
+
+      rco <$ drco;
+
+      cm <@ MCO.o((rco, m));
+
+      (sigfl, sk) <@ FL_KU_DSS.sign(sk, cm);
+
+      sig <- (rco, sigfl);
+
+      comps <- rcons comps (cm, (rco, m));
+      qs <- rcons qs m;
+      
+      return sig;
+    }
+
+    (* 
+      Check whether given message m is fresh, i.e., whether m is not contained in
+      the list of oracle queries qs 
+    *)
+    proc fresh(m : msg_al_t) : bool = {
+      return ! m \in qs;
+    }
+    
+    (* Get the number of oracle queries, i.e., the size of the oracle query list qs *)
+    proc nr_queries() : int = {
+      return size qs;
+    }
+    
+    proc compressions() : (msg_fl_t * (rco_t * msg_al_t)) list = {
+      return comps;
+    }
+}.
+
+local module EF_CMA_RO_Coll = {
+  var coll : bool
+  
+  proc main() = {
+    var pk : pk_al_t;
+    var sk : sk_al_t;
+    var m : msg_al_t;
+    var sig : sig_al_t;
+    var is_valid, is_fresh : bool;
+    var rco : rco_t;
+    var cm : msg_fl_t;
+    var comps : (msg_fl_t * (rco_t * msg_al_t)) list;
+    
+    (* Initialize (hash) random oracle *)
+    MCO.init();
+    
+    (* Generate a key pair using the considered signature scheme *)
+    (pk, sk) <@ AL_KU_DSS(FL_KU_DSS).keygen();
+
+    (* Initialize the signing oracle with the generated secret key *)
+    O_CMA_Coll.init(sk);
+
+    (*
+      Ask the adversary to forge a signature for any message (and provide both the
+      message and the signature) given the public key pk and access to a signing oracle 
+      that it can query an unlimited number of times
+    *)
+    (m, sig) <@ A(O_CMA_Coll, MCO).forge(pk);
+
+    (* 
+      Verify (w.r.t. message m) the signature sig provided by the adversary 
+      using the verification algorithm of the considered signature scheme 
+    *)
+    is_valid <@ AL_KU_DSS(FL_KU_DSS).verify(pk, m, sig);
+
+    (* 
+      Check whether message for which the adversary forged a signature is fresh 
+      (i.e., check whether message is not included in the list of messages for which 
+      the adversary received signatures through an oracle query)
+    *)
+    is_fresh <@ O_CMA_Coll.fresh(m);
+    
+    (* Collision check *)
+    rco <- sig.`1;
+    cm <@ MCO.o(rco, m);
+    comps <@ O_CMA_Coll.compressions();
+    
+    coll <- assoc comps cm <> None;
+    
+    (* 
+      Success iff
+      (1) "is_valid": the forged signature provided by the adversary is valid, and
+      (2) "is_fresh": the message for which the adversary forged a signature is fresh.
+    *)
+    return is_valid /\ is_fresh;
+  }
+}.
+
+local equiv Equiv_EFCMARO_EFCMAROColl :
+  EF_CMA_RO(AL_KU_DSS(FL_KU_DSS), A, O_CMA, MCO).main ~ EF_CMA_RO_Coll.main : ={glob FL_KU_DSS, glob A} ==> ={res}.
+proof.
+proc; inline *.
+seq 19 20 : (={is_valid, is_fresh}); last by wp.
+seq 8 9 : (={glob FL_KU_DSS, pk, m, sig, ERO.m} /\ ={qs}(O_CMA, O_CMA_Coll)); last by sim.
+call (: ={glob FL_KU_DSS, ERO.m} /\ ={sk, qs}(O_CMA, O_CMA_Coll)); first by proc.
++ proc; inline{1} 1. 
+  by wp; call (: true); call (: ={ERO.m}); auto.
+by wp; call (: true); while (={w, ERO.m}); auto.
+qed.
+
+local lemma EFCMAROColl_CRRO &m:
+  Pr[EF_CMA_RO_Coll.main() @ &m : res /\ EF_CMA_RO_Coll.coll]
+  <=
+  Pr[CR_RO(R_EFCMARO_CRRO(FL_KU_DSS, A), MCO).main() @ &m : res].
+proof.
+byequiv => //.
+proc; inline{1} 6; inline{2} 2.
+conseq (: _ ==> is_fresh{1} /\ EF_CMA_RO_Coll.coll{1} => kx{2} <> kx'{2} /\ y{2} = y'{2}); 1: by smt().
+seq 4 4 : (   ={sk, comps}(O_CMA_Coll, R_EFCMARO_CRRO.O_CMA_R_EFCMARO_CRRO) 
+           /\ (glob MCO){1} = (glob ERO){2}
+           /\ m{1} = mal'{2}
+           /\ sig{1} = sig'{2}
+           /\ (forall (mfl : msg_fl_t) (rmal : rco_t * msg_al_t), (mfl, rmal) \in O_CMA_Coll.comps{1}
+                 => mfl = oget (MCO.m{1}.[rmal]))
+           /\ (forall (msg : msg_fl_t), assoc O_CMA_Coll.comps{1} msg <> None 
+                 => (oget (assoc O_CMA_Coll.comps{1} msg)).`2 \in O_CMA_Coll.qs{1})).
++ call (:   ={glob FL_KU_DSS}   
+         /\ ={sk, comps}(O_CMA_Coll, R_EFCMARO_CRRO.O_CMA_R_EFCMARO_CRRO)
+         /\ (glob MCO){1} = (glob ERO){2}
+         /\ (forall (mfl : msg_fl_t) (rmal : rco_t * msg_al_t), (mfl, rmal) \in O_CMA_Coll.comps{1}
+              => mfl = oget (MCO.m{1}.[rmal]))
+         /\ (forall (msg : msg_fl_t), assoc O_CMA_Coll.comps{1} msg <> None
+              => (oget (assoc O_CMA_Coll.comps{1} msg)).`2 \in O_CMA_Coll.qs{1})).
+  - by proc; skip.
+  - proc; inline *.
+    wp; call (: true); wp; rnd; skip => /> &1 &2 comps_def compsqs_rel rco _.
+    split => [mfl rmal | mfl]; rewrite mem_rcons /=.
+    * by move=> -[[-> <-] //|]; apply comps_def.
+    rewrite -cats1 assoc_cat.
+    case (mfl \in unzip1 R_EFCMARO_CRRO.O_CMA_R_EFCMARO_CRRO.comps{2}) => assin.
+    * by move/compsqs_rel => ->.
+    by move/assocTP => /= ->; rewrite assoc_cons.
+  inline{1} 3; inline{2} 3.
+  wp; call (: true).
+  call (: true ==> (glob MCO){1} = (glob ERO){2}); last by skip.
+  proc.
+  by while (={w, ERO.m}); auto.
+inline *; wp.
+call{1} (: true ==> true); 1: by apply FL_KU_DSS_verify_ll.
+wp; skip => /> &1 &2 comps_def compsqs_rel malnin assnnone.
+split; 1: by rewrite negb_and; right => /#.
+pose cm := oget ERO.m{2}.[sig'{2}.`1, mal'{2}].
+move: (comps_def cm (oget (assoc R_EFCMARO_CRRO.O_CMA_R_EFCMARO_CRRO.comps{2} cm)) _).
++ by move/assocTP: assnnone; apply assoc_get_mem. 
+by move=> {3}-> /#.
+qed.
+
+
+local lemma EFCMAROColl_METCRRO &m:
+  Pr[EF_CMA_RO_Coll.main() @ &m : res /\ EF_CMA_RO_Coll.coll]
+  <=
+  Pr[M_ETCR_RO(R_EFCMARO_METCRRO(FL_KU_DSS, A), O_METCR, MCO).main() @ &m : res].
+proof.
+byequiv => //.
+proc; inline{2} 3.
+conseq (: _ ==> is_fresh{1} /\ EF_CMA_RO_Coll.coll{1} => 0 <= i{2} < nrts{2} /\ x{2} <> x'{2} /\ y{2} = y'{2}); 1: by smt().
+seq 4 5 : (   ={sk, comps}(O_CMA_Coll, R_EFCMARO_METCRRO.O_CMA_R_EFCMARO_METCRRO) 
+           /\ (glob MCO){1} = (glob ERO){2}
+           /\ m{1} = mal'{2}
+           /\ sig{1} = sig'{2}
+           /\ unzip2 R_EFCMARO_METCRRO.O_CMA_R_EFCMARO_METCRRO.comps{2} = O_METCR.ts{2}
+           /\ (forall (mfl : msg_fl_t) (rmal : rco_t * msg_al_t), (mfl, rmal) \in O_CMA_Coll.comps{1}
+                 => mfl = oget (MCO.m{1}.[rmal]))
+           /\ (forall (msg : msg_fl_t), assoc O_CMA_Coll.comps{1} msg <> None 
+                 => (oget (assoc O_CMA_Coll.comps{1} msg)).`2 \in O_CMA_Coll.qs{1})).
++ call (:   ={glob FL_KU_DSS}   
+         /\ ={sk, comps}(O_CMA_Coll, R_EFCMARO_METCRRO.O_CMA_R_EFCMARO_METCRRO)
+         /\ (glob MCO){1} = (glob ERO){2}
+         /\ unzip2 R_EFCMARO_METCRRO.O_CMA_R_EFCMARO_METCRRO.comps{2} = O_METCR.ts{2}
+         /\ (forall (mfl : msg_fl_t) (rmal : rco_t * msg_al_t), (mfl, rmal) \in O_CMA_Coll.comps{1}
+              => mfl = oget (MCO.m{1}.[rmal]))
+         /\ (forall (msg : msg_fl_t), assoc O_CMA_Coll.comps{1} msg <> None
+              => (oget (assoc O_CMA_Coll.comps{1} msg)).`2 \in O_CMA_Coll.qs{1})).
+  - by proc; skip.
+  - proc; inline *.
+    wp; call (: true); wp; rnd; wp; skip => /> &1 &2 comps_def compsqs_rel rco _.
+    split; last split => [ mfl rmal | mfl].
+    * by rewrite map_rcons.
+    * by rewrite mem_rcons /= => -[[-> <-] // |]; apply comps_def.
+    rewrite mem_rcons -cats1 assoc_cat /=.
+    case (mfl \in unzip1 R_EFCMARO_METCRRO.O_CMA_R_EFCMARO_METCRRO.comps{2}) => assin.
+    * by move/compsqs_rel => ->.
+    by move/assocTP => /= ->; rewrite assoc_cons.
+  inline *.
+  wp; call (: true).
+  by while (={w, ERO.m}); auto.
+inline *; wp.
+call{1} (: true ==> true); 1: by apply FL_KU_DSS_verify_ll.
+wp; skip => /> &1 &2 comps_def compsqs_rel malnin assnnone.
+split; 1: split => [| _]; 1: by rewrite index_ge0.
++ have ->:
+    size (unzip2 R_EFCMARO_METCRRO.O_CMA_R_EFCMARO_METCRRO.comps{2})
+    =
+    size (unzip1 R_EFCMARO_METCRRO.O_CMA_R_EFCMARO_METCRRO.comps{2}).
+  - by rewrite 2!size_map.
+  by rewrite index_mem -assocTP.
+split; 1: by rewrite nth_onth -assoc_zip 1:2!size_map // zip_unzip /#.
+pose cm := oget ERO.m{2}.[sig'{2}.`1, mal'{2}].
+move: (comps_def cm (oget (assoc R_EFCMARO_METCRRO.O_CMA_R_EFCMARO_METCRRO.comps{2} cm)) _).
++ by move/assocTP: assnnone; apply assoc_get_mem. 
+move=> {3}->; congr; congr.
+rewrite eq_sym -{1}(zip_unzip R_EFCMARO_METCRRO.O_CMA_R_EFCMARO_METCRRO.comps{2}).
+by rewrite assoc_zip 1:2!size_map // nth_onth /oget /#.
+qed.
 
 end section Proof_EFCMA_RO_ALKUDSS.
